rename

lib/Base/PackedInts.s.dfy
@@ -3,7 +3,7 @@ include "../Base/NativeTypes.s.dfy"
 module PackedInts {
   import opened NativeTypes
 
-  function {:opaque} unpackLittleEndianUint32(s: seq<byte>) : uint32
+  function {:opaque} unpack_LittleEndian_Uint32(s: seq<byte>) : uint32
   requires |s| == 4
   {
     (s[0] as uint32)
@@ -12,7 +12,7 @@ module PackedInts {
     + (s[3] as uint32 * 0x1_00_00_00)
   }
 
-  function {:opaque} unpackLittleEndianUint64(s: seq<byte>) : uint64
+  function {:opaque} unpack_LittleEndian_Uint64(s: seq<byte>) : uint64
   requires |s| == 8
   {
     (s[0] as uint64)
@@ -25,38 +25,44 @@ module PackedInts {
     + (s[7] as uint64 * 0x1_00_00_00_00_00_00_00)
   }
 
-  function {:opaque} unpackLittleEndianUint32Seq(
+  function {:opaque} unpack_LittleEndian_Uint32_Seq(
       packed: seq<byte>,
       len: int) : (unpacked: seq<uint32>)
   requires |packed| == len * 4
   ensures |unpacked| == len
   ensures forall i | 0 <= i < len ::
-      unpacked[i] == unpackLittleEndianUint32(packed[4*i .. 4*i + 4])
+      unpacked[i] == unpack_LittleEndian_Uint32(packed[4*i .. 4*i + 4])
   {
     assert forall i | 0 <= i < len - 1 ::
       packed[4*i .. 4*i + 4] == packed[..4*(len-1)][4*i .. 4*i + 4];
 
     if len == 0 then [] else (
-      unpackLittleEndianUint32Seq(packed[..4*(len-1)], len-1)
-        + [unpackLittleEndianUint32(packed[4*(len-1)..4*len])]
+      unpack_LittleEndian_Uint32_Seq(packed[..4*(len-1)], len-1)
+        + [unpack_LittleEndian_Uint32(packed[4*(len-1)..4*len])]
     )
   }
 
-  function {:opaque} unpackLittleEndianUint64Seq(
+  function {:opaque} unpack_LittleEndian_Uint64_Seq(
       packed: seq<byte>,
       len: int) : (unpacked: seq<uint64>)
   requires |packed| == len * 8
   ensures |unpacked| == len
   ensures forall i | 0 <= i < len ::
-      unpacked[i] == unpackLittleEndianUint64(packed[8*i .. 8*i + 8])
+      unpacked[i] == unpack_LittleEndian_Uint64(packed[8*i .. 8*i + 8])
   {
     assert forall i | 0 <= i < len - 1 ::
       packed[8*i .. 8*i + 8] == packed[..8*(len-1)][8*i .. 8*i + 8];
 
     if len == 0 then [] else (
-      unpackLittleEndianUint64Seq(packed[..8*(len-1)], len-1)
-        + [unpackLittleEndianUint64(packed[8*(len-1)..8*len])]
+      unpack_LittleEndian_Uint64_Seq(packed[..8*(len-1)], len-1)
+        + [unpack_LittleEndian_Uint64(packed[8*(len-1)..8*len])]
     )
   }
 
+  method {:axiom} Pack_LittleEndian_Uint64_into_Array(i: uint64, ar: array<byte>, idx: uint64)
+  requires 0 <= idx
+  requires idx as int + 8 <= ar.Length
+  ensures forall i | 0 <= i < idx :: ar[i] == old(ar[i])
+  ensures unpack_LittleEndian_Uint64(ar[idx .. idx + 8]) == i
+  ensures forall i | idx as int + 8 <= i < ar.Length :: ar[i] == old(ar[i])
 }
